\documentclass{article}
\usepackage{amsmath}
\usepackage{amssymb}
\begin{document}
\noindent Let a, b, c $\in \mathbb{Z}$\\

\noindent(a) $ (a | b) \  \land \ ( b | c ) \Rightarrow  (a | c) $\\
$(a | b) \land (b|c) \Rightarrow \exists (k, k') \in \mathbb{Z}^2
\ |\  (b = ka) \land (c = k'b)$\\
$\Rightarrow c = k'ka\blacksquare$\\

\noindent(b) $ (a|b) \land (b|a) \Rightarrow a = \pm b$\\
$(a|b) \land (b|a) \Rightarrow \exists (k, k') \in \mathbb{Z}^2
\ |\ (a = kb) \land (b = k'a)$\\
$\Rightarrow k'a = ka$\\
$\Rightarrow (k = k' = 1) \lor (k = k' = -1) \blacksquare$\\

\noindent(c) $(a | b) \land (a|c) \Rightarrow (a|(b+c))
\land (a|(b-c))$\\
$(a | b) \land (a|c) \Rightarrow (b + c = a(k + k'))
\land (b - c = a(k - k'))\blacksquare$

\end{document}
